

## Лагранж

Если
1. $f(x)$ непрерывна на $[a;b]$ 
2. Дифференцируема на $(a,b)$

То
$\exists \phi \in(a;b): \dfrac{{f(b)-f(a)}}{b-a}=f'(\phi)$

### Докво

Вспомогательная функция
$F(x):=f(x)-\dfrac{{f(b)-f(a)}}{b-a}(x-a)$

1. $F(a)=f(a)-\dfrac{{f(b)-f(a)}}{b-a}\cancelto{ \ 0 }{ (a-a) }=0$
2. $F(b)=f(b)-\dfrac{{f(b)-f(a)}}{b-a}(b-a)=f(a)$
   
По теореме Ролля $\exists \phi \in(a;b):F'(\phi)=0$

$F'(x)=f'(x)-\dfrac{{f(b)-f(a)}}{b-a}\cdot1$
$F'(\phi)=f'(\phi)-\dfrac{{f(b)-f(a)}}{b-a}=0$

$f'(\phi)=\dfrac{{f(b)-f(a)}}{b-a}$

## Коши

Пусть
1. Функции $y=y(t);x=x(t)$
2. Непрерывны на $[a;b]$
3. Дифференцируемы на $[a;b]$
4. $x'(t)\neq0$ на $[a;b]$
   
Тогда существует $\phi$
Такая, что $\dfrac{{y(b)-y(a)}}{x(b)-x(a)}=\dfrac{{y'(\phi)}}{x'(\phi)}$

### Докво

Возьмем вспомогательную 
$F(t)=x(t)(y(b)-y(a))-y(t)(x(b)-x(a))$

Разложить...

$F(a)=F(b)\implies$ по теореме Ролля $\exists \phi \in(a;b):F'(\phi)=0$

$x'(t)(y(b)-y(a))-y'(x(b)-x(a))=0$
$\dfrac{{y(b)-y(a)}}{x(b)-x(a)}=\dfrac{{y'(\phi)}}{x'(\phi)}$